new-backend/pat_to_closScript.sml
@@ -1,9 +1,9 @@
 open HolKernel boolLib boolSimps bossLib lcsymtacs miscLib intLib
 open rich_listTheory listTheory alistTheory finite_mapTheory pred_setTheory stringTheory integerTheory arithmeticTheory
-open patLangTheory callLangTheory
+open patLangTheory closLangTheory
 open astTheory semanticPrimitivesTheory
 open terminationTheory free_varsTheory compilerTerminationTheory
-val _ = new_theory"callLangProof"
+val _ = new_theory"pat_to_clos"
 
 (* TODO: move? *)
 val ALOOKUP_SNOC = store_thm("ALOOKUP_SNOC",
@@ -18,22 +18,22 @@ val ALOOKUP_GENLIST = store_thm("ALOOKUP_GENLIST",
   gen_tac >> Induct >> simp[GENLIST] >> rw[] >> fs[ALOOKUP_SNOC] >>
   rw[] >> fsrw_tac[ARITH_ss][])
 
-val tEval_MAP_Op_Const = store_thm("tEval_MAP_Op_Const",
+val cEval_MAP_Op_Const = store_thm("cEval_MAP_Op_Const",
   ``∀f env s ls.
-      tEval (MAP (λx. Op (Const (f x)) []) ls,env,s) =
+      cEval (MAP (λx. Op (Const (f x)) []) ls,env,s) =
       (Result (MAP (Number o f) ls),s)``,
   ntac 3 gen_tac >> Induct >>
-  simp[tEval_def] >>
-  simp[Once tEval_CONS] >>
-  simp[tEval_def,tEvalOp_def])
+  simp[cEval_def] >>
+  simp[Once cEval_CONS] >>
+  simp[cEval_def,cEvalOp_def])
 
-val tEval_REPLICATE_Op_AllocGlobal = store_thm("tEval_REPLICATE_Op_AllocGlobal",
-  ``∀n env s. tEval (REPLICATE n (Op AllocGlobal []),env,s) =
+val cEval_REPLICATE_Op_AllocGlobal = store_thm("cEval_REPLICATE_Op_AllocGlobal",
+  ``∀n env s. cEval (REPLICATE n (Op AllocGlobal []),env,s) =
               (Result (GENLIST (K(Number 0)) n),s with globals := s.globals ++ GENLIST (K NONE) n)``,
-  Induct >> simp[tEval_def,REPLICATE] >- (
-    simp[call_state_component_equality] ) >>
-  simp[Once tEval_CONS,tEval_def,tEvalOp_def,GENLIST_CONS] >>
-  simp[call_state_component_equality])
+  Induct >> simp[cEval_def,REPLICATE] >- (
+    simp[clos_state_component_equality] ) >>
+  simp[Once cEval_CONS,cEval_def,cEvalOp_def,GENLIST_CONS] >>
+  simp[clos_state_component_equality])
 
 val evaluate_list_pat_length = store_thm("evaluate_list_pat_length",
   ``∀ck env s es x vs.
@@ -44,7 +44,7 @@ val evaluate_list_pat_length = store_thm("evaluate_list_pat_length",
   rw[] >> res_tac)
 
 val bool_to_val_thm = store_thm("bool_to_val_thm",
-  ``bool_to_val b = callLang$Block (if b then 1 else 0) []``,
+  ``bool_to_val b = closLang$Block (if b then 1 else 0) []``,
   Cases_on`b`>>rw[bool_to_val_def])
 val bool_to_tag_thm = store_thm("bool_to_tag_thm",
   ``bool_to_tag b = if b then 1 else 0``,
@@ -82,7 +82,7 @@ val pComp_def = tDefine"pComp"`
   (pComp (Var_global_pat n) =
     Op (Global n) []) ∧
   (pComp (Fun_pat e) =
-    Fn 0 (pComp e)) ∧
+    Fn 0 [] (pComp e)) ∧
   (pComp (App_pat (Op_pat (Op_i2 Opapp)) es) =
     if LENGTH es ≠ 2 then Op Sub (MAP pComp es) else
     App NONE (pComp (EL 0 es)) (pComp (EL 1 es))) ∧
@@ -221,7 +221,7 @@ val pComp_def = tDefine"pComp"`
   (pComp (Seq_pat e1 e2) =
     Let [pComp e1;pComp e2] (Var 1)) ∧
   (pComp (Letrec_pat es e) =
-    Letrec 0 (MAP pComp es) (pComp e)) ∧
+    Letrec 0 [] (MAP pComp es) (pComp e)) ∧
   (pComp (Extend_global_pat n) =
    Let (REPLICATE n (Op AllocGlobal []))
      (Op (Cons unit_tag) []))`
@@ -236,7 +236,7 @@ val pComp_def = tDefine"pComp"`
 val _ = export_rewrites["pComp_def"]
 
 val v_to_Cv_def = tDefine"v_to_Cv"`
-  (v_to_Cv (Litv_pat (IntLit i)) = (Number i)) ∧
+  (v_to_Cv (Litv_pat (IntLit i)) = (Number i):clos_val) ∧
   (v_to_Cv (Litv_pat (Word8 w)) = (Number (&w2n w))) ∧
   (v_to_Cv (Litv_pat (Char c)) = (Number (& ORD c))) ∧
   (v_to_Cv (Litv_pat (StrLit s)) =
@@ -254,7 +254,7 @@ val v_to_Cv_def = tDefine"v_to_Cv"`
      rw[] >> res_tac >> fs[] >> simp[v_pat_size_def])
 val _ = export_rewrites["v_to_Cv_def"]
 
-val sv_to_Cref_def = Define`
+val sv_to_Cref_def = Define `
   (sv_to_Cref (Refv v) = ValueArray [v_to_Cv v]) ∧
   (sv_to_Cref (Varray vs) = ValueArray (MAP v_to_Cv vs)) ∧
   (sv_to_Cref (W8array bs) = ByteArray bs)`
@@ -265,7 +265,8 @@ val s_to_Cs_def = Define`
        refs := alist_to_fmap (GENLIST (λi. (i, sv_to_Cref (EL i s))) (LENGTH s));
        clock := c;
        code := FEMPTY;
-       output := "" |>`
+       output := "";
+       restrict_envs := F |>`
 
 val res_to_Cres_def = Define`
   (res_to_Cres f (Rval v) = Result (f v)) ∧
@@ -274,59 +275,63 @@ val res_to_Cres_def = Define`
   (res_to_Cres f (Rerr Rtype_error) = Error)`
 val _ = export_rewrites["res_to_Cres_def"]
 
-val do_eq_pat_call_equal = store_thm("do_eq_pat_call_equal",
+val do_eq_pat_clos_equal = store_thm("do_eq_pat_clos_equal",
   ``(∀v1 v2. do_eq_pat v1 v2 ≠ Eq_type_error ⇒
-      (do_eq_pat v1 v2 = call_equal (v_to_Cv v1) (v_to_Cv v2))) ∧
+      (do_eq_pat v1 v2 = clos_equal (v_to_Cv v1) (v_to_Cv v2))) ∧
     (∀vs1 vs2. do_eq_list_pat vs1 vs2 ≠ Eq_type_error ⇒
-      (do_eq_list_pat vs1 vs2 = call_equal_list (MAP v_to_Cv vs1) (MAP v_to_Cv vs2)))``,
+      (do_eq_list_pat vs1 vs2 = clos_equal_list (MAP v_to_Cv vs1) (MAP v_to_Cv vs2)))``,
   ho_match_mp_tac do_eq_pat_ind >>
-  simp[do_eq_pat_def,call_equal_def] >>
+  simp[do_eq_pat_def,clos_equal_def] >>
   conj_tac >- (
-    Cases >> Cases >> simp[lit_same_type_def,call_equal_def,ORD_11,bool_to_tag_thm] >>
+    Cases >> Cases >> simp[lit_same_type_def,clos_equal_def,ORD_11,bool_to_tag_thm] >>
     TRY(rw[] >> pop_assum mp_tac >> rw[] >> NO_TAC) >>
     qid_spec_tac`s'` >>
-    Induct_on`s` >> simp[LENGTH_NIL_SYM,call_equal_def] >> rw[] >>
+    Induct_on`s` >> simp[LENGTH_NIL_SYM,clos_equal_def] >> rw[] >>
     TRY (
       spose_not_then strip_assume_tac >> rw[] >> fs[] >> NO_TAC) >>
-    Cases_on`s'`>>fs[call_equal_def,ORD_11] >> rw[]) >>
+    Cases_on`s'`>>fs[clos_equal_def,ORD_11] >> rw[]) >>
   conj_tac >- rw[ETA_AX] >>
   conj_tac >- rw[ETA_AX] >>
   rw[] >>
   Cases_on`v1`>>fs[]>>TRY(Cases_on`l:lit`>>fs[])>>
   Cases_on`v2`>>fs[]>>TRY(Cases_on`l:lit`>>fs[])>>
-  fs[do_eq_pat_def,call_equal_def,lit_same_type_def,ORD_11,bool_to_tag_thm] >>
+  fs[do_eq_pat_def,clos_equal_def,lit_same_type_def,ORD_11,bool_to_tag_thm] >>
   rw[]>>fs[]>>rfs[ETA_AX]>>
   BasicProvers.CASE_TAC>>fs[]>>
   rw[]>>fs[]>>
   BasicProvers.CASE_TAC>>fs[])
 
-val call_to_list_correct = store_thm("call_to_list_correct",
-  ``∀ls. call_to_list (MAP (Number o $& o ORD) ls) =
+val clos_to_list_correct = store_thm("clos_to_list_correct",
+  ``∀ls. clos_to_list (MAP (Number o $& o ORD) ls) =
          v_to_Cv (char_list_to_v_pat ls)``,
-  Induct >> simp[call_to_list_def,char_list_to_v_pat_def])
+  Induct >> simp[clos_to_list_def,char_list_to_v_pat_def])
 
-val call_from_char_list_correct = store_thm("call_from_char_list_correct",
+val clos_from_char_list_correct = store_thm("clos_from_char_list_correct",
   ``∀v ls. (v_pat_to_char_list v = SOME ls) ⇒
-           (call_from_list (v_to_Cv v) = SOME (MAP (Number o $& o ORD) ls))``,
+           (clos_from_list (v_to_Cv v) = SOME (MAP (Number o $& o ORD) ls))``,
   ho_match_mp_tac v_pat_to_char_list_ind >>
-  simp[v_pat_to_char_list_def,call_from_list_def] >>
+  simp[v_pat_to_char_list_def,clos_from_list_def] >>
   rw[] >>
   Cases_on`v`>>fs[v_pat_to_char_list_def] >>
-  Cases_on`l`>>fs[v_pat_to_char_list_def,call_from_list_def] >>
+  Cases_on`l`>>fs[v_pat_to_char_list_def,clos_from_list_def] >>
   rw[]>>fs[]>>
-  Cases_on`h`>>fs[v_pat_to_char_list_def,call_from_list_def] >>
-  Cases_on`l`>>fs[v_pat_to_char_list_def,call_from_list_def] >>
-  Cases_on`t`>>fs[v_pat_to_char_list_def,call_from_list_def] >>
-  Cases_on`t'`>>fs[v_pat_to_char_list_def,call_from_list_def] >>
+  Cases_on`h`>>fs[v_pat_to_char_list_def,clos_from_list_def] >>
+  Cases_on`l`>>fs[v_pat_to_char_list_def,clos_from_list_def] >>
+  Cases_on`t`>>fs[v_pat_to_char_list_def,clos_from_list_def] >>
+  Cases_on`t'`>>fs[v_pat_to_char_list_def,clos_from_list_def] >>
   rw[]>>fs[]>>
   Cases_on`v_pat_to_char_list h`>>fs[]>> rw[])
 
-val call_from_list_correct = store_thm("call_from_list_correct",
+val clos_from_list_correct = store_thm("clos_from_list_correct",
   ``∀v ls. (v_to_list_pat v = SOME ls) ⇒
-           (call_from_list (v_to_Cv v) = SOME (MAP v_to_Cv ls))``,
+           (clos_from_list (v_to_Cv v) = SOME (MAP v_to_Cv ls))``,
   ho_match_mp_tac v_to_list_pat_ind >>
-  simp[v_to_list_pat_def,call_from_list_def] >>
+  simp[v_to_list_pat_def,clos_from_list_def] >>
   rw[] >> Cases_on`v_to_list_pat v`>>fs[]>> rw[])
+
+val s_to_Cs_restrict_envs = prove(
+  ``~(s_to_Cs s).restrict_envs``,
+  Cases_on `s` \\ Cases_on `q` \\ fs [s_to_Cs_def]);
 
 val pComp_correct = store_thm("pComp_correct",
   ``(∀ck env s e res. evaluate_pat ck env s e res ⇒
@@ -334,57 +339,57 @@ val pComp_correct = store_thm("pComp_correct",
        set (free_vars_pat e) ⊆ count (LENGTH env) ∧
        EVERY closed_pat env ∧ csg_closed_pat s ∧
        SND res ≠ Rerr Rtype_error ⇒
-       tEval ([pComp e],MAP v_to_Cv env,s_to_Cs s) =
+       cEval ([pComp e],MAP v_to_Cv env,s_to_Cs s) =
          (res_to_Cres (λv. [v_to_Cv v]) (SND res), s_to_Cs (FST res))) ∧
     (∀ck env s es res. evaluate_list_pat ck env s es res ⇒
        ck ∧
        set (free_vars_list_pat es) ⊆ count (LENGTH env) ∧
        EVERY closed_pat env ∧ csg_closed_pat s ∧
        SND res ≠ Rerr Rtype_error ⇒
-       tEval (MAP pComp es,MAP v_to_Cv env,s_to_Cs s) =
+       cEval (MAP pComp es,MAP v_to_Cv env,s_to_Cs s) =
          (res_to_Cres (MAP v_to_Cv) (SND res), s_to_Cs (FST res)))``,
   ho_match_mp_tac evaluate_pat_strongind >>
   strip_tac >- (
     Cases_on`l`>>
-    rw[tEval_def,tEvalOp_def] >>
-    simp[tEval_MAP_Op_Const,combinTheory.o_DEF] ) >>
-  strip_tac >- simp[tEval_def] >>
+    rw[cEval_def,cEvalOp_def] >>
+    simp[cEval_MAP_Op_Const,combinTheory.o_DEF] ) >>
+  strip_tac >- simp[cEval_def] >>
   strip_tac >- (
-    simp[tEval_def] >>
+    simp[cEval_def] >>
     Cases_on`err`>>simp[] ) >>
-  strip_tac >- simp[tEval_def] >>
+  strip_tac >- simp[cEval_def] >>
   strip_tac >- (
-    simp[tEval_def] >>
+    simp[cEval_def] >>
     rw[] >> first_x_assum match_mp_tac >>
     imp_res_tac evaluate_pat_closed >> rfs[] >>
     fs[SUBSET_DEF,PULL_EXISTS] >>
     Cases >> rw[] >> res_tac >>
     fsrw_tac[ARITH_ss][] ) >>
   strip_tac >- (
-    simp[tEval_def] >>
+    simp[cEval_def] >>
     Cases_on`err`>>simp[] ) >>
-  strip_tac >- simp[tEval_def,ETA_AX,tEvalOp_def] >>
+  strip_tac >- simp[cEval_def,ETA_AX,cEvalOp_def] >>
   strip_tac >- (
     Cases_on`err`>>
-    simp[tEval_def,ETA_AX,tEvalOp_def] ) >>
-  strip_tac >- simp[tEval_def,EL_MAP] >>
-  strip_tac >- simp[tEval_def] >>
+    simp[cEval_def,ETA_AX,cEvalOp_def] ) >>
+  strip_tac >- simp[cEval_def,EL_MAP] >>
+  strip_tac >- simp[cEval_def] >>
   strip_tac >- (
-    simp[tEval_def,tEvalOp_def] >>
+    simp[cEval_def,cEvalOp_def] >>
     Cases_on`s`>>simp[s_to_Cs_def,get_global_def,EL_MAP] ) >>
-  strip_tac >- simp[tEval_def] >>
-  strip_tac >- simp[tEval_def] >>
-  strip_tac >- simp[tEval_def,ETA_AX] >>
+  strip_tac >- simp[cEval_def] >>
+  strip_tac >- simp[cEval_def] >>
+  strip_tac >- simp[cEval_def,ETA_AX,s_to_Cs_restrict_envs,clos_env_def] >>
   strip_tac >- (
-    simp[tEval_def] >>
-    rw[tEval_def] >>
+    simp[cEval_def] >>
+    rw[cEval_def] >>
     imp_res_tac evaluate_list_pat_length >>
     Cases_on`vs`>>fs[do_opapp_pat_def] >>
     Cases_on`t`>>fs[do_opapp_pat_def] >>
     Cases_on`t'`>>fs[do_opapp_pat_def] >>
     Cases_on`es`>>fs[]>>
     Cases_on`t`>>fs[LENGTH_NIL]>>
-    fs[tEval_def] >>
+    fs[cEval_def] >>
     BasicProvers.CASE_TAC >> fs[] >> Cases_on`q`>>fs[]>>
     BasicProvers.CASE_TAC >> fs[] >> Cases_on`q`>>fs[]>>
     rw[dest_closure_def] >>
@@ -408,43 +413,43 @@ val pComp_correct = store_thm("pComp_correct",
     fs[MAP_GENLIST,combinTheory.o_DEF,ETA_AX] >>
     fsrw_tac[ETA_ss][] ) >>
   strip_tac >- (
-    simp[tEval_def] >>
-    rw[tEval_def] >>
+    simp[cEval_def] >>
+    rw[cEval_def] >>
     imp_res_tac evaluate_list_pat_length >>
     Cases_on`vs`>>fs[do_opapp_pat_def] >>
     Cases_on`t`>>fs[do_opapp_pat_def] >>
     Cases_on`t'`>>fs[do_opapp_pat_def] >>
     Cases_on`es`>>fs[]>>
     Cases_on`t`>>fs[LENGTH_NIL]>>
-    fs[tEval_def] >>
+    fs[cEval_def] >>
     BasicProvers.CASE_TAC >> fs[] >> Cases_on`q`>>fs[]>>
     BasicProvers.CASE_TAC >> fs[] >> Cases_on`q`>>fs[]>>
     rw[dest_closure_def] >>
     Cases_on`h`>>fs[check_loc_def,s_to_Cs_def,ETA_AX,dec_clock_def] >>
     rw[] >> rw[] >>
     fsrw_tac[ARITH_ss][] ) >>
-  strip_tac >- simp[tEval_def] >>
+  strip_tac >- simp[cEval_def] >>
   strip_tac >- (
-    simp[tEval_def] >> rw[] >>
+    simp[cEval_def] >> rw[] >>
     PairCases_on`s2` >>
     imp_res_tac do_app_pat_cases >>
     fs[do_app_pat_def] >> rw[] >- (
-      Cases_on`z`>>fs[tEval_def,ETA_AX,tEvalOp_def] >>
-      rw[opn_lookup_def,call_equal_def,bool_to_val_thm] >>
+      Cases_on`z`>>fs[cEval_def,ETA_AX,cEvalOp_def] >>
+      rw[opn_lookup_def,clos_equal_def,bool_to_val_thm] >>
       TRY IF_CASES_TAC >> fs[] >> fsrw_tac[ARITH_ss][] >>
       BasicProvers.EVERY_CASE_TAC >> fs[] >>
       rw[prim_exn_pat_def,opn_lookup_def] )
     >- (
-      Cases_on`z`>>fs[tEval_def,ETA_AX,tEvalOp_def,bool_to_tag_thm,opb_lookup_def,bool_to_val_thm] >>
+      Cases_on`z`>>fs[cEval_def,ETA_AX,cEvalOp_def,bool_to_tag_thm,opb_lookup_def,bool_to_val_thm] >>
       simp[] >> rw[] >> COOPER_TAC )
     >- (
-      simp[tEval_def,ETA_AX,tEvalOp_def] >>
+      simp[cEval_def,ETA_AX,cEvalOp_def] >>
       Cases_on`do_eq_pat v1 v2 = Eq_type_error`>>fs[] >>
-      imp_res_tac do_eq_pat_call_equal >> fs[] >>
+      imp_res_tac do_eq_pat_clos_equal >> fs[] >>
       BasicProvers.CASE_TAC >> fs[] >> rw[bool_to_tag_thm,bool_to_val_thm] >>
       fsrw_tac[ARITH_ss][prim_exn_pat_def])
     >- (
-      simp[tEval_def,ETA_AX,tEvalOp_def] >>
+      simp[cEval_def,ETA_AX,cEvalOp_def] >>
       fs[store_assign_def,Once s_to_Cs_def] >>
       BasicProvers.CASE_TAC >- (
         imp_res_tac ALOOKUP_FAILS >> fs[MEM_GENLIST] ) >>
@@ -458,17 +463,17 @@ val pComp_correct = store_thm("pComp_correct",
       REWRITE_TAC[GSYM EL] >>
       simp[EL_LUPDATE] )
     >- (
-      simp[ETA_AX,tEval_def,tEvalOp_def] >>
+      simp[ETA_AX,cEval_def,cEvalOp_def] >>
       fs[store_lookup_def] >>
       imp_res_tac evaluate_list_pat_length >>
       Cases_on`es`>>fs[LENGTH_NIL] >>
-      simp[Once tEval_CONS,tEval_def,tEvalOp_def] >>
+      simp[Once cEval_CONS,cEval_def,cEvalOp_def] >>
       simp[s_to_Cs_def,ALOOKUP_GENLIST] >>
       rw[]>>fs[] >>
       Cases_on`EL n s21`>>fs[sv_to_Cref_def] >>
       rw[s_to_Cs_def] )
     >- (
-      simp[ETA_AX,tEval_def,tEvalOp_def] >>
+      simp[ETA_AX,cEval_def,cEvalOp_def] >>
       fs[store_alloc_def,LET_THM] >>
       rpt BasicProvers.VAR_EQ_TAC >>
       simp[s_to_Cs_def,fmap_eq_flookup,FLOOKUP_UPDATE] >>
@@ -482,12 +487,12 @@ val pComp_correct = store_thm("pComp_correct",
       simp[ALOOKUP_GENLIST] >>
       rw[] >> simp[EL_APPEND1,EL_APPEND2,sv_to_Cref_def] )
     >- (
-      simp[tEval_def,ETA_AX,tEvalOp_def,s_to_Cs_def,get_global_def,EL_MAP] >>
+      simp[cEval_def,ETA_AX,cEvalOp_def,s_to_Cs_def,get_global_def,EL_MAP] >>
       Cases_on`EL idx s22`>>fs[] >>
       rpt BasicProvers.VAR_EQ_TAC >>
       simp[s_to_Cs_def,LUPDATE_MAP] )
     >- (
-      simp[tEval_def,ETA_AX,tEvalOp_def,bool_to_val_thm] >>
+      simp[cEval_def,ETA_AX,cEvalOp_def,bool_to_val_thm] >>
       fs[store_alloc_def,LET_THM] >>
       Cases_on`n<0`>>fs[prim_exn_pat_def] >- rw[] >>
       `0 ≤ n` by COOPER_TAC >>
@@ -506,7 +511,7 @@ val pComp_correct = store_thm("pComp_correct",
       rw[] >> simp[EL_APPEND1,EL_LENGTH_APPEND,sv_to_Cref_def] >>
       metis_tac[INT_ABS_EQ_ID])
     >- (
-      simp[tEval_def,ETA_AX,tEvalOp_def,bool_to_val_thm] >>
+      simp[cEval_def,ETA_AX,cEvalOp_def,bool_to_val_thm] >>
       fs[store_lookup_def,LET_THM] >>
       Cases_on`lnum < LENGTH s21`>>fs[] >>
       Cases_on`i < 0` >> fs[] >- (
@@ -522,14 +527,14 @@ val pComp_correct = store_thm("pComp_correct",
       simp[ALOOKUP_GENLIST,sv_to_Cref_def] >>
       rw[s_to_Cs_def] )
     >- (
-      simp[tEval_def,ETA_AX,tEvalOp_def] >>
+      simp[cEval_def,ETA_AX,cEvalOp_def] >>
       fs[store_lookup_def] >>
       simp[s_to_Cs_def,ALOOKUP_GENLIST] >>
       Cases_on`n < LENGTH s21`>>fs[]>>
       Cases_on`EL n s21`>>fs[sv_to_Cref_def] >>
       rw[s_to_Cs_def] )
     >- (
-      simp[tEval_def,ETA_AX,tEvalOp_def,bool_to_val_thm] >>
+      simp[cEval_def,ETA_AX,cEvalOp_def,bool_to_val_thm] >>
       fs[store_lookup_def,LET_THM] >>
       Cases_on`lnum < LENGTH s21`>>fs[] >>
       Cases_on`i < 0` >> fs[] >- (
@@ -553,35 +558,35 @@ val pComp_correct = store_thm("pComp_correct",
       imp_res_tac evaluate_list_pat_length >> fs[] )
     >- ( Cases_on`es`>>fs[LENGTH_NIL] )
     >- (
-      simp[tEval_def,ETA_AX,tEvalOp_def,bool_to_val_thm,prim_exn_pat_def] )
+      simp[cEval_def,ETA_AX,cEvalOp_def,bool_to_val_thm,prim_exn_pat_def] )
     >- (
-      simp[tEval_def,ETA_AX,tEvalOp_def,bool_to_val_thm,prim_exn_pat_def] >>
+      simp[cEval_def,ETA_AX,cEvalOp_def,bool_to_val_thm,prim_exn_pat_def] >>
       Cases_on`n < 0` >> fs[] >>
       `255 < n` by COOPER_TAC >> simp[])
     >- (
-      simp[tEval_def,ETA_AX,tEvalOp_def,bool_to_val_thm,prim_exn_pat_def] >> fs[] >>
+      simp[cEval_def,ETA_AX,cEvalOp_def,bool_to_val_thm,prim_exn_pat_def] >> fs[] >>
       `¬(255 < n)` by COOPER_TAC >> simp[] >>
       `ABS n = n` by COOPER_TAC >>
       `Num n < 256` by COOPER_TAC >>
       `0 ≤ n` by COOPER_TAC >>
       simp[ORD_CHR,INT_OF_NUM])
     >- (
-      Cases_on`z`>>fs[tEval_def,ETA_AX,tEvalOp_def,bool_to_tag_thm,opb_lookup_def,bool_to_val_thm] >>
+      Cases_on`z`>>fs[cEval_def,ETA_AX,cEvalOp_def,bool_to_tag_thm,opb_lookup_def,bool_to_val_thm] >>
       simp[] >> rw[] >> COOPER_TAC )
     >- (
-      simp[tEval_def,ETA_AX,tEvalOp_def] >>
-      simp[call_to_list_correct,IMPLODE_EXPLODE_I])
+      simp[cEval_def,ETA_AX,cEvalOp_def] >>
+      simp[clos_to_list_correct,IMPLODE_EXPLODE_I])
     >- (
-      simp[tEval_def,ETA_AX,tEvalOp_def] >>
-      imp_res_tac call_from_char_list_correct >>
+      simp[cEval_def,ETA_AX,cEvalOp_def] >>
+      imp_res_tac clos_from_char_list_correct >>
       simp[IMPLODE_EXPLODE_I])
-    >- ( simp[tEval_def,ETA_AX,tEvalOp_def] )
+    >- ( simp[cEval_def,ETA_AX,cEvalOp_def] )
     >- (
-      simp[tEval_def,ETA_AX,tEvalOp_def] >>
-      imp_res_tac call_from_list_correct >>
+      simp[cEval_def,ETA_AX,cEvalOp_def] >>
+      imp_res_tac clos_from_list_correct >>
       simp[])
     >- (
-      simp[tEval_def,ETA_AX,tEvalOp_def,bool_to_val_thm] >>
+      simp[cEval_def,ETA_AX,cEvalOp_def,bool_to_val_thm] >>
       Cases_on`i < 0` >> fs[LET_THM] >- (
         rw[prim_exn_pat_def] ) >>
       `0 ≤ i` by COOPER_TAC >>
@@ -591,9 +596,9 @@ val pComp_correct = store_thm("pComp_correct",
         rw[s_to_Cs_def,prim_exn_pat_def] ) >>
       rpt BasicProvers.VAR_EQ_TAC >>
       simp[EL_MAP] )
-    >- ( simp[tEval_def,ETA_AX,tEvalOp_def])
+    >- ( simp[cEval_def,ETA_AX,cEvalOp_def])
     >- (
-      simp[tEval_def,ETA_AX,tEvalOp_def,bool_to_val_thm] >>
+      simp[cEval_def,ETA_AX,cEvalOp_def,bool_to_val_thm] >>
       fs[store_alloc_def,LET_THM] >>
       Cases_on`n<0`>>fs[prim_exn_pat_def] >- rw[] >>
       `0 ≤ n` by COOPER_TAC >>
@@ -611,7 +616,7 @@ val pComp_correct = store_thm("pComp_correct",
       simp[REPLICATE_GENLIST,MAP_GENLIST] >>
       metis_tac[INT_ABS_EQ_ID])
     >- (
-      simp[tEval_def,ETA_AX,tEvalOp_def,bool_to_val_thm] >>
+      simp[cEval_def,ETA_AX,cEvalOp_def,bool_to_val_thm] >>
       fs[store_lookup_def,LET_THM] >>
       Cases_on`lnum < LENGTH s21`>>fs[] >>
       Cases_on`i < 0` >> fs[] >- (
@@ -627,14 +632,14 @@ val pComp_correct = store_thm("pComp_correct",
       simp[ALOOKUP_GENLIST,sv_to_Cref_def,EL_MAP] >>
       rw[s_to_Cs_def] )
     >- (
-      simp[tEval_def,ETA_AX,tEvalOp_def] >>
+      simp[cEval_def,ETA_AX,cEvalOp_def] >>
       fs[store_lookup_def] >>
       simp[s_to_Cs_def,ALOOKUP_GENLIST] >>
       Cases_on`n < LENGTH s21`>>fs[]>>
       Cases_on`EL n s21`>>fs[sv_to_Cref_def] >>
       rw[s_to_Cs_def] )
     >- (
-      simp[tEval_def,ETA_AX,tEvalOp_def,bool_to_val_thm] >>
+      simp[cEval_def,ETA_AX,cEvalOp_def,bool_to_val_thm] >>
       fs[store_lookup_def,LET_THM] >>
       Cases_on`lnum < LENGTH s21`>>fs[] >>
       Cases_on`i < 0` >> fs[] >- (
@@ -653,46 +658,46 @@ val pComp_correct = store_thm("pComp_correct",
       simp[ALOOKUP_GENLIST] >>
       rw[] >> fs[EL_LUPDATE,sv_to_Cref_def,LUPDATE_MAP])
     >- (
-      simp[tEval_def,ETA_AX,tEvalOp_def,bool_to_val_thm,bool_to_tag_thm] )
-    >- ( simp[tEval_def,ETA_AX,tEvalOp_def,EL_MAP] )) >>
-  strip_tac >- simp[tEval_def] >>
+      simp[cEval_def,ETA_AX,cEvalOp_def,bool_to_val_thm,bool_to_tag_thm] )
+    >- ( simp[cEval_def,ETA_AX,cEvalOp_def,EL_MAP] )) >>
+  strip_tac >- simp[cEval_def] >>
   strip_tac >- (
-    simp[tEval_def] >> rw[] >>
-    Cases_on`op`>>simp[tEval_def,ETA_AX] >>
+    simp[cEval_def] >> rw[] >>
+    Cases_on`op`>>simp[cEval_def,ETA_AX] >>
     TRY( Cases_on`err`>>fs[] >> NO_TAC) >>
-    Cases_on`o'`>>simp[tEval_def,ETA_AX] >>
+    Cases_on`o'`>>simp[cEval_def,ETA_AX] >>
     TRY( Cases_on`err`>>fs[] >> NO_TAC) >>
-    Cases_on`o''`>>simp[tEval_def,ETA_AX] >>
-    rw[tEval_def] >>
+    Cases_on`o''`>>simp[cEval_def,ETA_AX] >>
+    rw[cEval_def] >>
     TRY( Cases_on`err`>>fs[] >> NO_TAC) >>
-    TRY(Cases_on`o'`>>simp[tEval_def,ETA_AX] >>
+    TRY(Cases_on`o'`>>simp[cEval_def,ETA_AX] >>
         Cases_on`err`>>fs[] >> NO_TAC) >>
     TRY(
       CHANGED_TAC(REWRITE_TAC[GSYM SNOC_APPEND]) >>
-      simp[Once tEval_SNOC] >>
+      simp[Once cEval_SNOC] >>
       Cases_on`err`>>fs[] >> NO_TAC) >>
     Cases_on`es`>>fs[LENGTH_NIL] >>
     Cases_on`t`>>fs[LENGTH_NIL] >>
-    TRY(CHANGED_TAC(fs[Once tEval_CONS]) >>
-        BasicProvers.CASE_TAC>>fs[]>>Cases_on`q`>>fs[tEval_def]>>rw[]>>
+    TRY(CHANGED_TAC(fs[Once cEval_CONS]) >>
+        BasicProvers.CASE_TAC>>fs[]>>Cases_on`q`>>fs[cEval_def]>>rw[]>>
         Cases_on`err`>>fs[]>>
-        BasicProvers.CASE_TAC>>fs[]>>Cases_on`q`>>fs[tEval_def]>>
+        BasicProvers.CASE_TAC>>fs[]>>Cases_on`q`>>fs[cEval_def]>>
         NO_TAC) >>
     Cases_on`err`>>fs[]) >>
   strip_tac >- (
-    simp[tEval_def] >>
+    simp[cEval_def] >>
     rw[] >>
     Cases_on`v`>>fs[]>>rw[]>>fs[do_if_pat_def]>>
     Cases_on`l`>>fs[]>>
     Cases_on`b`>>fs[]>>rw[]>>
     imp_res_tac evaluate_pat_closed >>fs[]) >>
-  strip_tac >- simp[tEval_def] >>
+  strip_tac >- simp[cEval_def] >>
   strip_tac >- (
-    simp[tEval_def] >> rw[] >>
+    simp[cEval_def] >> rw[] >>
     imp_res_tac evaluate_pat_closed >>fs[] >>
     Cases_on`err`>>fs[] ) >>
   strip_tac >- (
-    simp[tEval_def] >> rw[] >>
+    simp[cEval_def] >> rw[] >>
     qpat_assum`X ⇒ Y`mp_tac >>
     discharge_hyps >- (
       imp_res_tac evaluate_pat_closed >>fs[] >>
@@ -701,9 +706,9 @@ val pComp_correct = store_thm("pComp_correct",
       fsrw_tac[ARITH_ss][]) >>
     simp[] ) >>
   strip_tac >- (
-    simp[tEval_def] >> Cases_on`err`>>simp[] ) >>
+    simp[cEval_def] >> Cases_on`err`>>simp[] ) >>
   strip_tac >- (
-    simp[tEval_def] >> rw[] >> fs[] >>
+    simp[cEval_def] >> rw[] >> fs[] >>
     qpat_assum`X ⇒ Y`mp_tac >>
     discharge_hyps >- (
       imp_res_tac evaluate_pat_closed >>fs[] ) >>
@@ -712,10 +717,10 @@ val pComp_correct = store_thm("pComp_correct",
     Cases_on`r`>>fs[]>>simp[]>>
     Cases_on`e''`>>simp[]) >>
   strip_tac >- (
-    simp[tEval_def] >>
+    simp[cEval_def] >>
     Cases_on`err`>>simp[] ) >>
   strip_tac >- (
-    simp[tEval_def] >>
+    simp[cEval_def] >>
     rw[] >> fs[] >>
     qpat_assum`X ⇒ Y`mp_tac >>
     discharge_hyps >- (
@@ -725,23 +730,24 @@ val pComp_correct = store_thm("pComp_correct",
       fs[MEM_FLAT,MEM_MAP,PULL_EXISTS] >>
       rw[] >> res_tac >> fs[] >> simp[] >>
       fs[EVERY_MEM] ) >>
-    rw[build_rec_env_pat_def,build_recc_def,MAP_GENLIST,combinTheory.o_DEF,ETA_AX,MAP_MAP_o] >>
+    rw[build_rec_env_pat_def,build_recc_def,MAP_GENLIST,s_to_Cs_restrict_envs,
+       combinTheory.o_DEF,ETA_AX,MAP_MAP_o,clos_env_def] >>
     fsrw_tac[ETA_ss][] ) >>
   strip_tac >- (
-    simp[tEval_def] >>
-    simp[tEval_REPLICATE_Op_AllocGlobal,tEvalOp_def] >>
+    simp[cEval_def] >>
+    simp[cEval_REPLICATE_Op_AllocGlobal,cEvalOp_def] >>
     Cases_on`s`>>simp[s_to_Cs_def,MAP_GENLIST,combinTheory.o_DEF,combinTheory.K_DEF] ) >>
-  strip_tac >- simp[tEval_def] >>
+  strip_tac >- simp[cEval_def] >>
   strip_tac >- (
-    simp[tEval_def] >> rw[] >>
-    simp[Once tEval_CONS] >>
+    simp[cEval_def] >> rw[] >>
+    simp[Once cEval_CONS] >>
     imp_res_tac evaluate_pat_closed >> fs[] ) >>
   strip_tac >- (
-    simp[tEval_def] >> rw[] >> fs[] >>
-    simp[Once tEval_CONS] >>
+    simp[cEval_def] >> rw[] >> fs[] >>
+    simp[Once cEval_CONS] >>
     Cases_on`err`>>fs[]) >>
-  simp[tEval_def] >> rw[] >>
-  simp[Once tEval_CONS] >>
+  simp[cEval_def] >> rw[] >>
+  simp[Once cEval_CONS] >>
   imp_res_tac evaluate_pat_closed >> fs[] >>
   Cases_on`err`>>fs[])
 
@@ -771,10 +777,10 @@ val code_locs_def = tDefine "code_locs" `
      let c1 = code_locs [x1] in
      let c2 = code_locs [x2] in
          c1++c2) /\
-  (code_locs [Fn loc x1] =
+  (code_locs [Fn loc vs x1] =
      let c1 = code_locs [x1] in
        loc::c1) /\
-  (code_locs [Letrec loc fns x1] =
+  (code_locs [Letrec loc vs fns x1] =
      let c1 = code_locs fns in
      let c2 = code_locs [x1] in
      GENLIST ($+ loc) (LENGTH fns) ++ c1 ++ c2) /\
@@ -784,7 +790,7 @@ val code_locs_def = tDefine "code_locs" `
        c1 ++ c2) /\
   (code_locs [Call dest xs] =
      code_locs xs)`
- (WF_REL_TAC `measure (call_exp1_size)`
+ (WF_REL_TAC `measure (clos_exp1_size)`
   \\ REPEAT STRIP_TAC \\ DECIDE_TAC);
 
 val code_locs_cons = store_thm("code_locs_cons",
@@ -820,13 +826,13 @@ val renumber_code_locs_def = tDefine "renumber_code_locs" `
      let (n,x1) = renumber_code_locs n x1 in
      let (n,x2) = renumber_code_locs n x2 in
        (n,App loc_opt x1 x2)) /\
-  (renumber_code_locs n (Fn loc x1) =
+  (renumber_code_locs n (Fn loc vs x1) =
      let (m,x1) = renumber_code_locs (n+1) x1 in
-       (m,Fn n x1)) /\
-  (renumber_code_locs n (Letrec loc fns x1) =
+       (m,Fn n vs x1)) /\
+  (renumber_code_locs n (Letrec loc vs fns x1) =
      let (m,fns) = renumber_code_locs_list (n+LENGTH fns) fns in
      let (m,x1) = renumber_code_locs m x1 in
-     (m,Letrec n fns x1)) /\
+     (m,Letrec n vs fns x1)) /\
   (renumber_code_locs n (Handle x1 x2) =
      let (n,x1) = renumber_code_locs n x1 in
      let (n,x2) = renumber_code_locs n x2 in
@@ -834,7 +840,7 @@ val renumber_code_locs_def = tDefine "renumber_code_locs" `
   (renumber_code_locs n (Call dest xs) =
      let (n,xs) = renumber_code_locs_list n xs in
      (n,Call dest xs))`
- (WF_REL_TAC `inv_image $< (λx. case x of INL p => call_exp1_size (SND p) | INR p => call_exp_size (SND p))`);
+ (WF_REL_TAC `inv_image $< (λx. case x of INL p => clos_exp1_size (SND p) | INR p => clos_exp_size (SND p))`);
 
 val renumber_code_locs_ind = theorem"renumber_code_locs_ind"
 
